update loops

proof/TableWalk/CodeProof/table_walk_lock_unlock.v
@@ -128,6 +128,207 @@ Section CodeProof.
                                          (Tcons tulong Tnil) tvoid cc_default).
     Local Opaque set_wi_index_spec.
 
+  Fixpoint table_walk_lock_unlock_loop0 (n: nat) (l: Z) (tbl: Pointer) (last_tbl: Pointer) (map_addr: Z) (adt: RData) :=
+    match n with
+    | O => Some (l, tbl, last_tbl, adt)
+    | S n' =>
+      match table_walk_lock_unlock_loop0 n' l tbl last_tbl map_addr adt with
+      | Some (l, (tbl_base, tbl_ofst), (last_tbl_base, last_tbl_ofst), adt) =>
+        rely is_int l; rely is_int tbl_ofst; rely is_int last_tbl_ofst;
+        when null == is_null_spec (tbl_base, tbl_ofst) adt;
+        rely is_int null;
+        if null =? 0 then
+          when' idx == addr_to_idx_spec (VZ64 map_addr) (VZ64 l) adt;
+          rely is_int64 idx;
+          when'' tbl_base, tbl_ofst, adt == find_next_level_idx_spec (tbl_base, tbl_ofst) (VZ64 idx) adt;
+          rely is_int tbl_ofst;
+          when null == is_null_spec (tbl_base, tbl_ofst) adt;
+          rely is_int null;
+          if null =? 0 then
+            when adt == granule_lock_spec (tbl_base, tbl_ofst) adt;
+            when adt == granule_unlock_spec (last_tbl_base, last_tbl_ofst) adt;
+            Some (l + 1, (tbl_base, tbl_ofst), (tbl_base, tbl_ofst), adt)
+          else
+            when adt == granule_unlock_spec (last_tbl_base, last_tbl_ofst) adt;
+            Some (l + 1, (tbl_base, tbl_ofst), (last_tbl_base, last_tbl_ofst), adt)
+        else Some (l + 1, (tbl_base, tbl_ofst), (last_tbl_base, last_tbl_ofst), adt)
+      | _ => None
+      end
+    end.
+
+  Definition table_walk_lock_unlock_spec0 (g_rd: Pointer) (map_addr: Z64) (level: Z64) (adt: RData) : option RData :=
+    match map_addr, level with
+    | VZ64 map_addr, VZ64 level =>
+      when'' rd_base, rd_ofst, adt == granule_map_spec g_rd SLOT_RD adt;
+      rely is_int rd_ofst;
+      when'' g_root_base, g_root_ofst == get_rd_g_rtt_spec (rd_base, rd_ofst) adt;
+      rely is_int g_root_ofst;
+      when adt == buffer_unmap_spec (rd_base, rd_ofst) adt;
+      when adt == granule_lock_spec (g_root_base, g_root_ofst) adt;
+      match table_walk_lock_unlock_loop0 (Z.to_nat level) 0 (g_root_base, g_root_ofst) (g_root_base, g_root_ofst) map_addr adt with
+      | Some (l, (tbl_base, tbl_ofst), (last_tbl_base, last_tbl_ofst), adt) =>
+        rely is_int l; rely is_int tbl_ofst; rely is_int last_tbl_ofst;
+        when adt == set_wi_g_llt_spec (tbl_base, tbl_ofst) adt;
+        when' idx == addr_to_idx_spec (VZ64 map_addr) (VZ64 level) adt;
+        rely is_int64 idx;
+        when adt == set_wi_index_spec (VZ64 idx) adt;
+        Some adt
+      | _ => None
+      end
+    end.
+
+    Ltac solve_func64 val :=
+      try unfold Monad.bind; try unfold ret; simpl;
+      match goal with
+      | [|- match ?v with | Some _ => _ | None => None end = _] =>
+          replace v with (Some (VZ64 (Int64.unsigned (Int64.repr val))))
+      end.
+
+    Ltac solve_func val :=
+      try unfold Monad.bind; try unfold ret; simpl;
+      match goal with
+      | [|- match ?v with | Some _ => _ | None => None end = _] =>
+          replace v with (Some (Int.unsigned (Int.repr val)))
+      end.
+
+    Lemma table_walk_lock_unlock_body_correct:
+      forall m d d' env le g_rd_base g_rd_offset map_addr level
+             (Henv: env = PTree.empty _)
+             (Hinv: high_level_invariant d)
+             (HPTg_rd: PTree.get _g_rd le = Some (Vptr g_rd_base (Int.repr g_rd_offset)))
+             (HPTmap_addr: PTree.get _map_addr le = Some (Vlong map_addr))
+             (HPTlevel: PTree.get _level le = Some (Vlong level))
+             (Hspec: table_walk_lock_unlock_spec0 (g_rd_base, g_rd_offset) (VZ64 (Int64.unsigned map_addr)) (VZ64 (Int64.unsigned level)) d = Some d'),
+           exists le', (exec_stmt ge env le ((m, d): mem) table_walk_lock_unlock_body E0 le' (m, d') Out_normal).
+    Proof.
+      solve_code_proof Hspec table_walk_lock_unlock_body.
+      get_loop_body. clear_hyp.
+      set (Hloop := C8). simpl; solve_proof_low.
+      remember
+        (PTree.set _last_tbl (Vptr p3 (Int.repr z0))
+            (PTree.set _tbl (Vptr p3 (Int.repr z0))
+              (PTree.set _t'3 (Vptr p3 (Int.repr z0))
+                  (PTree.set _g_root (Vptr p3 (Int.repr z0))
+                    (PTree.set _t'2 (Vptr p3 (Int.repr z0))
+                        (PTree.set _rd (Vptr p1 (Int.repr z))
+                          (PTree.set _t'1 (Vptr p1 (Int.repr z))
+                              (PTree.set _last_level (Vlong (Int64.repr 0))
+                                (PTree.set _l (Vlong (Int64.repr 0)) le)))))))))
+            as le_loop.
+      remember (Int64.unsigned level) as num.
+      set (P := fun le0 m0 => m0 = (m, r1) /\ le0 = le_loop).
+      set (Q := fun (le0: temp_env) m0 => m0 = (m, r2) /\
+                                            le0 ! _map_addr = Some (Vlong map_addr) /\
+                                            le0 ! _level = Some (Vlong level) /\
+                                            le0 ! _tbl = Some (Vptr p9 (Int.repr z2))).
+      set (Inv := fun le0 m0 n => exists l' tbl_base' tbl_ofst' last_tbl_base' last_tbl_ofst' adt',
+                      table_walk_lock_unlock_loop0 (Z.to_nat (num - n)) 0
+                                                   (p3, z0) (p3, z0) (Int64.unsigned map_addr) r1 =
+                        Some (Int64.unsigned l', (tbl_base', tbl_ofst'),
+                               (last_tbl_base', last_tbl_ofst'), adt') /\
+                        Int64.unsigned l' = num - n /\
+                        m0 = (m, adt') /\ 0 <= n /\ n <= num /\
+                        le0 ! _l = Some (Vlong l') /\
+                        le0 ! _map_addr = Some (Vlong map_addr) /\
+                        le0 ! _level = Some (Vlong level) /\
+                        le0 ! _tbl = Some (Vptr tbl_base' (Int.repr tbl_ofst')) /\
+                        le0 ! _last_tbl = Some (Vptr last_tbl_base' (Int.repr last_tbl_ofst'))).
+      assert(loop_succ: forall N, Z.of_nat N <= num -> exists l' tbl_base' tbl_ofst' last_tbl_base' last_tbl_ofst' adt',
+                  table_walk_lock_unlock_loop0 (Z.to_nat (num - Z.of_nat N)) 0
+                                               (p3, z0) (p3, z0) (Int64.unsigned map_addr) r1 =
+                    Some (Int64.unsigned l', (tbl_base', tbl_ofst'),
+                           (last_tbl_base', last_tbl_ofst'), adt')).
+        { add_int64 Hloop z1; try somega.
+          add_int Hloop z2; try somega.
+          add_int Hloop z3; try somega.
+          induction N. rewrite Z.sub_0_r. rewrite Hloop. intros. repeat eexists; reflexivity.
+          intros. erewrite loop_ind_sub1 in IHN; try omega.
+          rewrite Nat2Z.inj_succ, succ_plus_1 in H.
+          assert(Hcc: Z.of_nat N <= num) by omega.
+          apply IHN in Hcc. destruct Hcc as (? & ? & ? & ? & ? & ? & Hnext).
+          Local Opaque Z.of_nat. simpl in Hnext. clear Heqle_loop.
+          simpl_func Hnext;
+            try add_int64' z4; try somega; try add_int' z6; try somega;
+            try add_int' z7; try somega; repeat eexists. }
+        assert (T: LoopProofSimpleWhile.t (external_calls_ops := CompatExternalCalls.compatlayer_extcall_ops L) cond body ge (PTree.empty _) P Q).
+        { apply LoopProofSimpleWhile.make with (W:=Z) (lt:=fun z1 z2 => (0 <= z2 /\ z1 < z2)) (I:=Inv).
+          - apply Zwf_well_founded.
+          - unfold P, Inv. intros ? ? CC. destruct CC as [CC1 CC2].
+            rewrite CC2 in *. exists num.
+            replace (num - num) with 0 by omega. simpl.
+            exists (Int64.repr 0). eexists. eexists.
+            eexists. eexists. eexists.
+            rewrite Heqnum. rewrite Heqle_loop.
+            repeat eexists; first [reflexivity|assumption|solve_proof_low].
+          - intros ? ? ? I. unfold Inv in I.
+            destruct I as (? & ? & ? & ? & ? & ? & ? & ? & ? & ? & ? & ? & ? & ? & ? & ?).
+            set (Hnow := H).
+            rewrite Heqbody, Heqcond in *.
+            destruct (n >? 0) eqn:Hn; bool_rel.
+            + eexists. eexists. split_and.
+              * solve_proof_low.
+              * solve_proof_low.
+              * intro CC. inversion CC.
+              * assert(Hlx: Z.of_nat (Z.to_nat (n-1)) <= num) by (rewrite Z2Nat.id; omega).
+                apply loop_succ in Hlx. rewrite Z2Nat.id in Hlx; try omega.
+                intro. destruct Hlx as (? & ? & ? & ? & ? & ? & Hnext). duplicate Hnext.
+                rewrite loop_nat_sub1 in Hnext; try somega.
+                simpl in Hnext. rewrite Hnow in Hnext.
+                autounfold in Hnext; repeat simpl_hyp Hnext;
+                  repeat destruct_con; bool_rel; contra; inversion Hnext.
+                rewrite H12 in *. rewrite H13 in *. rewrite H14 in *.
+                rewrite H15 in *. rewrite H16 in *.
+                 eexists; eexists; split.
+                repeat big_vcgen. solve_func z4. reflexivity.
+                symmetry. sstep. assumption. somega.
+                solve_proof_low. simpl.
+                solve_proof_low. solve_proof_low.
+                solve_proof_low.
+                exists (n-1); split. split; solve_proof_low.
+                solve_proof_low; unfold Inv; repeat eexists; first[eassumption|solve_proof_low].
+
+                rewrite H12 in *. rewrite H13 in *. rewrite H14 in *.
+                rewrite H15 in *. rewrite H16 in *.
+                eexists; eexists; split.
+                repeat big_vcgen. solve_func z4. reflexivity.
+                symmetry. sstep. assumption. somega.
+                solve_proof_low. simpl.
+                solve_proof_low. solve_proof_low.
+                solve_proof_low.
+                exists (n-1); split. split; solve_proof_low.
+                solve_proof_low; unfold Inv; repeat eexists; first[eassumption|solve_proof_low].
+
+                rewrite H12 in *. rewrite H13 in *. rewrite H14 in *.
+                rewrite H15 in *. rewrite H16 in *.
+                eexists; eexists; split.
+                repeat big_vcgen. solve_func z4. reflexivity.
+                symmetry. sstep. assumption. somega.
+                solve_proof_low. simpl.
+                solve_proof_low. solve_proof_low.
+                solve_proof_low.
+                exists (n-1); split. split; solve_proof_low.
+                solve_proof_low; unfold Inv; repeat eexists; first[eassumption|solve_proof_low].
+            + eexists. eexists. split_and.
+              * solve_proof_low.
+              * solve_proof_low.
+              * intro. unfold Q.
+                assert (n=0) by omega. clear Heqle_loop. subst.
+                sstep. rewrite Hloop in Hnow. inv Hnow.
+                split_and; first[reflexivity|solve_proof_low].
+              * intro CC. inversion CC. }
+        assert (Pre: P le_loop (m, r1)) by (split; reflexivity).
+        pose proof (LoopProofSimpleWhile.termination _ _ _ _ _ _ T _ (m, r1) Pre) as LoopProof.
+        destruct LoopProof as (le' & m' & (exec & Post)).
+        unfold exec_stmt in exec. rewrite Heqle_loop in exec.
+        unfold Q in Post. destruct Post as (Post & Hle'). rewrite Post in exec.
+
+      destruct Hle' as (? & ? & ?).
+      eexists; solve_proof_low.
+      solve_func64 z5. reflexivity.
+      symmetry. sstep. rewrite <- Heqnum. assumption.
+      sstep. sstep. assumption. somega.
+    Qed.
+
   End BodyProof.
 
 End CodeProof.
