proof/RealmSyncHandler/Specs/handle_realm_rsi.v
@@ -12,7 +12,55 @@ Local Open Scope Z_scope.
 Section Spec.
 
   Definition handle_realm_rsi_spec (rec: Pointer) (adt: RData) : option (RData * Z) :=
-    None.
+	  when' function_id == get_rec_regs_spec rec 0 adt;
+	  when' arg1 == get_rec_regs_spec rec 1 adt;
+	  when' arg2 == get_rec_regs_spec rec 2 adt;
+	  when' arg3 == get_rec_regs_spec rec 3 adt;
+    rely is_int64 function_id; rely is_int64 arg1; rely is_int64 arg2; rely is_int64 arg3;
+    if function_id =? SMC_RSI_ABI_VERSION then
+		  when adt == set_rec_regs_spec rec 1 (VZ64 RSI_ABI_VERSION) adt;
+		  when adt == set_rec_regs_spec rec 0 (VZ64 STATUS_SUCCESS) adt;
+      Some (adt, 1)
+    else
+      if ((function_id >=? SMC32_PSCI_BASE) && (function_id <=? SMC32_PSCI_MAX)) ||
+         ((function_id >=? SMC64_PSCI_BASE) && (function_id <=? SMC64_PSCI_MAX))
+      then
+		    when adt == psci_rsi_spec rec function_id (VZ64 arg1) (VZ64 arg2) (VZ64 arg3) adt;
+        when' x0 == get_psci_result_x0_spec adt;
+        rely is_int64 x0;
+		    when adt == set_rec_regs_spec rec 0 (VZ64 x0) adt;
+        when' x1 == get_psci_result_x1_spec adt;
+        rely is_int64 x1;
+		    when adt == set_rec_regs_spec rec 1 (VZ64 x1) adt;
+        when' x2 == get_psci_result_x2_spec adt;
+        rely is_int64 x2;
+		    when adt == set_rec_regs_spec rec 2 (VZ64 x2) adt;
+        when' x3 == get_psci_result_x3_spec adt;
+        rely is_int64 x3;
+		    when adt == set_rec_regs_spec rec 3 (VZ64 x3) adt;
+        when forward == get_psci_result_forward_psci_call_spec adt;
+        rely is_int forward;
+        if forward =? 1 then
+			    when adt == set_rec_run_exit_reason_spec (VZ64 EXIT_REASON_PSCI) adt;
+			    when adt == set_rec_run_gprs_spec 0 (VZ64 function_id) adt;
+          when' x1 == get_psci_result_forward_x1_spec adt;
+          rely is_int64 x1;
+          when adt == set_rec_run_gprs_spec 1 (VZ64 x1) adt;
+          when' x2 == get_psci_result_forward_x2_spec adt;
+          rely is_int64 x2;
+          when adt == set_rec_run_gprs_spec 2 (VZ64 x2) adt;
+          when' x3 == get_psci_result_forward_x3_spec adt;
+          rely is_int64 x3;
+          when adt == set_rec_run_gprs_spec 3 (VZ64 x3) adt;
+          when adt == set_rec_run_gprs_spec 4 (VZ64 0) adt;
+          when adt == set_rec_run_gprs_spec 5 (VZ64 0) adt;
+          when adt == set_rec_run_gprs_spec 6 (VZ64 0) adt;
+          Some (adt, 0)
+        else
+          Some (adt, 1)
+		  else
+		    when adt == set_rec_regs_spec rec 0 (VZ64 SMC_RETURN_UNKNOWN_FUNCTION) adt;
+        Some (adt, 1).
 
 End Spec.
 
