proof/TableAux/CodeProof/table_has_destroyed.v
@@ -46,6 +46,108 @@ Section CodeProof.
                                       (Tcons Tptr (Tcons tulong Tnil)) tulong cc_default).
     Local Opaque pgte_read_spec.
 
+
+  Lemma table_has_destroyed_body_correct:
+      forall m d env le table_base table_offset res
+             (Henv: env = PTree.empty _)
+             (Hinv: high_level_invariant d)
+             (HPTtable: PTree.get _table le = Some (Vptr table_base (Int.repr table_offset)))
+             (Hspec: table_has_destroyed_spec0 (table_base, table_offset) d = Some (Int.unsigned res)),
+           exists le', (exec_stmt ge env le ((m, d): mem) table_has_destroyed_body E0 le' (m, d) (Out_return (Some (Vint res, tuint)))).
+    Proof.
+      solve_code_proof Hspec table_has_destroyed_body;  try solve [eexists; solve_proof_low].
+      get_loop_body. clear_hyp.
+      set (Hloop := C). simpl; solve_proof_low.
+      remember (PTree.set _i (Vlong (Int64.repr 0)) le)  as le_loop.
+      remember 512 as num.
+      set (P := fun le0 m0 => m0 = (m, d) /\ le0 = le_loop).
+      set (Q := fun (le0: temp_env) m0 => m0 = (m, d)).
+      set (Inv := fun le0 m0 n => exists i' res',
+                      table_has_destroyed_loop0 (Z.to_nat (num - n)) 0 0 (table_base, table_offset) d
+                      = Some (Int64.unsigned i', Int.unsigned res') /\ Int64.unsigned i' = num - n /\
+                        m0 = (m, d) /\ 0 <= n /\ n <= num /\ le0 ! _i = Some (Vlong i') /\
+                        le0 ! _table = Some (Vptr table_base (Int.repr table_offset))).
+      assert(loop_succ: forall N, Z.of_nat N <= num -> exists i' res',
+                  table_has_destroyed_loop0 (Z.to_nat (num - Z.of_nat N)) 0 0 (table_base, table_offset) d
+                  = Some (Int64.unsigned i', Int.unsigned res')).
+      { add_int64 Hloop z; try somega.
+        induction N. rewrite Z.sub_0_r. rewrite Hloop. intros. repeat eexists; reflexivity.
+        intros. erewrite loop_ind_sub1 in IHN; try omega.
+        rewrite Nat2Z.inj_succ, succ_plus_1 in H.
+        assert(Hcc: Z.of_nat N <= num) by omega.
+        apply IHN in Hcc. destruct Hcc as (? & ? & Hnext).
+        Local Opaque Z.of_nat. simpl in Hnext. clear Heqle_loop.
+        simpl_func Hnext; try add_int64' z0; try somega; try add_int' z1; try somega; repeat eexists. }
+      assert (T: LoopProofSimpleWhile.t (external_calls_ops := CompatExternalCalls.compatlayer_extcall_ops L) cond body ge (PTree.empty _) P Q).
+      { apply LoopProofSimpleWhile.make with (W:=Z) (lt:=fun z1 z2 => (0 <= z2 /\ z1 < z2)) (I:=Inv).
+        - apply Zwf_well_founded.
+        - unfold P, Inv. intros ? ? CC. destruct CC as [CC1 CC2].
+          rewrite CC2 in *. exists num.
+          replace (num - num) with 0 by omega. simpl.
+          exists (Int64.repr 0). exists (Int.repr 0).
+          rewrite Heqnum. rewrite Heqle_loop.
+          repeat eexists; first [reflexivity|assumption|solve_proof_low].
+        - intros ? ? ? I. unfold Inv in I. destruct I as (? & ? & ? & ? & ? & ? & ? & ? & ?).
+          set (Hnow := H).
+          rewrite Heqbody, Heqcond in *.
+          destruct (n >? 0) eqn:Hn; bool_rel.
+          + eexists. eexists. split_and.
+            * solve_proof_low.
+            * solve_proof_low.
+            * intro CC. inversion CC.
+            * assert(Hlx: Z.of_nat (Z.to_nat (n-1)) <= num) by (rewrite Z2Nat.id; omega).
+              apply loop_succ in Hlx. rewrite Z2Nat.id in Hlx; try omega.
+              intro. destruct Hlx as (? & ? & Hnext). duplicate Hnext.
+              rewrite loop_nat_sub1 in Hnext; try somega.
+              simpl in Hnext. rewrite Hnow in Hnext.
+              autounfold in Hnext; repeat simpl_hyp Hnext;
+                repeat destruct_con; bool_rel; contra; inversion Hnext.
+              rewrite H8, H9 in *; eexists; eexists; split.
+              set (ZZ := Int64.repr z1).
+              replace z1 with (Int64.unsigned ZZ) in C2.
+              solve_proof_low.
+              match goal with
+              | [|- match ?v with Some _ => _ | None => None end = _] =>
+                  replace v with (Some (VZ64 (Int64.unsigned ZZ)))
+              end.
+              reflexivity.
+              somega. replace ZZ with (Int64.repr z1) by reflexivity.
+              solve_proof_low.
+              exists (n-1); split. split; solve_proof_low.
+              solve_proof_low; unfold Inv; repeat eexists; first[eassumption|solve_proof_low].
+              rewrite H8, H9. rewrite D. solve_proof_low.
+              rewrite H8. solve_proof_low.
+
+              rewrite H8, H9 in *; eexists; eexists; split.
+              set (ZZ := Int64.repr z1).
+              replace z1 with (Int64.unsigned ZZ) in C2.
+              solve_proof_low.
+              match goal with
+              | [|- match ?v with Some _ => _ | None => None end = _] =>
+                  replace v with (Some (VZ64 (Int64.unsigned ZZ)))
+              end.
+              reflexivity.
+              somega. somega. somega.
+              replace ZZ with (Int64.repr z1) by reflexivity.
+              solve_proof_low.
+              exists (n-1); split. split; solve_proof_low.
+              solve_proof_low; unfold Inv; repeat eexists; first[eassumption|solve_proof_low].
+          + eexists. eexists. split_and.
+            * solve_proof_low.
+            * solve_proof_low.
+            * intro. unfold Q.
+              assert (n=0) by omega. clear Heqle_loop. subst.
+              sstep. rewrite Hloop in Hnow. inv Hnow.
+              split_and; first[reflexivity|solve_proof_low].
+            * intro CC. inversion CC. }
+        assert (Pre: P le_loop (m, d)) by (split; reflexivity).
+        pose proof (LoopProofSimpleWhile.termination _ _ _ _ _ _ T _ (m, d) Pre) as LoopProof.
+        destruct LoopProof as (le' & m' & (exec & Post)).
+        unfold exec_stmt in exec. rewrite Heqle_loop in exec.
+        unfold Q in Post. rewrite Post in exec.
+        eexists; solve_proof_low.
+    Qed.
+
   End BodyProof.
 
 End CodeProof.
