proof/TableAux/CodeProof/table_maps_block.v
@@ -64,6 +64,168 @@ Section CodeProof.
                                                   (Tcons tulong (Tcons tulong Tnil)) tuint cc_default).
     Local Opaque addr_is_level_aligned_spec.
 
+
+    Ltac solve_func64 val :=
+      try unfold Monad.bind; try unfold ret; simpl;
+      match goal with
+      | [|- match ?v with | Some _ => _ | None => None end = _] =>
+          replace v with (Some (VZ64 (Int64.unsigned (Int64.repr val))))
+      end.
+
+    Ltac solve_func val :=
+      try unfold Monad.bind; try unfold ret; simpl;
+      match goal with
+      | [|- match ?v with | Some _ => _ | None => None end = _] =>
+          replace v with (Some (Int.unsigned (Int.repr val)))
+      end.
+
+    Lemma table_maps_block_body_correct:
+      forall m d env le table_base table_offset level ipa_state res
+             (Henv: env = PTree.empty _)
+             (Hinv: high_level_invariant d)
+             (HPTtable: PTree.get _table le = Some (Vptr table_base (Int.repr table_offset)))
+             (HPTlevel: PTree.get _level le = Some (Vlong level))
+             (HPTipa_state: PTree.get _ipa_state le = Some (Vlong ipa_state))
+             (Hspec: table_maps_block_spec0 (table_base, table_offset) (VZ64 (Int64.unsigned level)) (VZ64 (Int64.unsigned ipa_state)) d = Some (Int.unsigned res)),
+           exists le', (exec_stmt ge env le ((m, d): mem) table_maps_block_body E0 le' (m, d) (Out_return (Some (Vint res, tuint)))).
+    Proof.
+      solve_code_proof Hspec table_maps_block_body.
+      - eexists. repeat big_vcgen.
+        solve_func64 z0. reflexivity.
+        symmetry. repeat sstep. assumption. somega.
+        solve_func64 z2. reflexivity.
+        symmetry. repeat sstep.
+        rewrite C8. reflexivity.
+        somega. somega. somega. somega.
+        solve_proof_low.
+        simpl. solve_proof_low.
+      - get_loop_body. clear_hyp.
+        set (Hloop := C11). simpl; solve_proof_low.
+        remember
+            (PTree.set _i (Vint (Int.repr 0))
+                (PTree.set _ret (Vint (Int.repr 1))
+                  (PTree.set _t'5 (Vint (Int.repr z3))
+                      (PTree.set _base_pa (Vlong (Int64.repr z2))
+                        (PTree.set _t'2 (Vlong (Int64.repr z2))
+                            (PTree.set _pgte (Vlong (Int64.repr z0))
+                              (PTree.set _t'1 (Vlong (Int64.repr z0)) le)))))))
+            as le_loop.
+        remember 512 as num.
+        set (P := fun le0 m0 => m0 = (m, d) /\ le0 = le_loop).
+        set (Q := fun (le0: temp_env) m0 => m0 = (m, d) /\ le0 ! _ret = Some (Vint res)).
+        set (Inv := fun le0 m0 n => exists i' ret',
+                        table_maps_block_loop0 (Z.to_nat (num - n)) 0 1 (table_base, table_offset) z2
+                                               (Int64.unsigned level) (Int64.unsigned ipa_state) d =
+                          Some (Int.unsigned i', Int.unsigned ret') /\ Int.unsigned i' = num - n /\
+                          m0 = (m, d) /\ 0 <= n /\ n <= num /\ le0 ! _i = Some (Vint i') /\
+                          le0 ! _table = Some (Vptr table_base (Int.repr table_offset)) /\
+                          le0 ! _level = Some (Vlong level) /\
+                          le0 ! _ipa_state = Some (Vlong ipa_state) /\
+                          le0 ! _ret = Some (Vint ret') /\
+                          le0 ! _base_pa = Some (Vlong (Int64.repr z2))).
+        assert(loop_succ: forall N, Z.of_nat N <= num -> exists i' ret',
+                    table_maps_block_loop0 (Z.to_nat (num - Z.of_nat N)) 0 1
+                                           (table_base, table_offset) z2
+                                           (Int64.unsigned level) (Int64.unsigned ipa_state) d =
+                      Some (Int.unsigned i', Int.unsigned ret')).
+        { add_int Hloop z4; try somega.
+          induction N. rewrite Z.sub_0_r. rewrite Hloop. intros. repeat eexists; reflexivity.
+          intros. erewrite loop_ind_sub1 in IHN; try omega.
+          rewrite Nat2Z.inj_succ, succ_plus_1 in H.
+          assert(Hcc: Z.of_nat N <= num) by omega.
+          apply IHN in Hcc. destruct Hcc as (? & ? & Hnext).
+          Local Opaque Z.of_nat. simpl in Hnext. clear Heqle_loop.
+          simpl_func Hnext; try add_int' z; try somega; try add_int' z1; try somega; repeat eexists. }
+        assert (T: LoopProofSimpleWhile.t (external_calls_ops := CompatExternalCalls.compatlayer_extcall_ops L) cond body ge (PTree.empty _) P Q).
+        { apply LoopProofSimpleWhile.make with (W:=Z) (lt:=fun z1 z2 => (0 <= z2 /\ z1 < z2)) (I:=Inv).
+          - apply Zwf_well_founded.
+          - unfold P, Inv. intros ? ? CC. destruct CC as [CC1 CC2].
+            rewrite CC2 in *. exists num.
+            replace (num - num) with 0 by omega. simpl.
+            exists (Int.repr 0). exists (Int.repr 1).
+            rewrite Heqnum. rewrite Heqle_loop.
+            repeat eexists; first [reflexivity|assumption|solve_proof_low].
+          - intros ? ? ? I. unfold Inv in I.
+            destruct I as (? & ? & ? & ? & ? & ? & ? & ? & ? & ? & ? & ? & ?).
+            set (Hnow := H).
+            rewrite Heqbody, Heqcond in *.
+            destruct (n >? 0) eqn:Hn; bool_rel.
+            + eexists. eexists. split_and.
+              * solve_proof_low.
+              * solve_proof_low.
+              * intro CC. inversion CC.
+              * assert(Hlx: Z.of_nat (Z.to_nat (n-1)) <= num) by (rewrite Z2Nat.id; omega).
+                apply loop_succ in Hlx. rewrite Z2Nat.id in Hlx; try omega.
+                intro. destruct Hlx as (? & ? & Hnext). duplicate Hnext.
+                rewrite loop_nat_sub1 in Hnext; try somega.
+                simpl in Hnext. rewrite Hnow in Hnext.
+                autounfold in Hnext; repeat simpl_hyp Hnext;
+                  repeat destruct_con; bool_rel; contra; inversion Hnext.
+                rewrite H12, H13 in *; eexists; eexists; split.
+                repeat big_vcgen.
+                solve_func64 z1. reflexivity.
+                symmetry. repeat sstep. assumption. somega.
+                solve_proof_low. somega. somega. somega. somega. somega. somega.
+                somega. somega. simpl.
+                solve_proof_low. solve_proof_low.
+                solve_proof_low. somega.
+                exists (n-1); split. split; solve_proof_low.
+                solve_proof_low; unfold Inv; repeat eexists; first[eassumption|solve_proof_low].
+                rewrite <- (Int.repr_unsigned x2). rewrite <- H13.
+                rewrite Int.repr_unsigned. assumption.
+
+                rewrite H12, H13 in *; eexists; eexists; split.
+                repeat big_vcgen.
+                solve_func64 z1. reflexivity.
+                symmetry. repeat sstep. assumption. somega.
+                solve_proof_low. somega. somega. somega. somega. somega. somega.
+                somega. somega. simpl.
+                solve_proof_low. solve_proof_low.
+                solve_proof_low. somega.
+                exists (n-1); split. split; solve_proof_low.
+                solve_proof_low; unfold Inv; repeat eexists; first[eassumption|solve_proof_low].
+                rewrite H12. rewrite H13. rewrite D. sstep. reflexivity.
+                rewrite H12. sstep. omega.
+
+                rewrite H12, H13 in *; eexists; eexists; split.
+                repeat big_vcgen.
+                solve_func64 z1. reflexivity.
+                symmetry. repeat sstep. assumption. somega.
+                solve_proof_low. somega. somega. somega. somega. somega. somega.
+                somega. somega. somega. somega.  simpl.
+                solve_proof_low. solve_proof_low.
+                solve_proof_low. somega.
+                exists (n-1); split. split; solve_proof_low.
+                solve_proof_low; unfold Inv; repeat eexists; first[eassumption|solve_proof_low].
+                rewrite H12. rewrite H13. rewrite D. sstep. reflexivity.
+                rewrite H12. sstep. omega.
+            + eexists. eexists. split_and.
+              * solve_proof_low.
+              * solve_proof_low.
+              * intro. unfold Q.
+                assert (n=0) by omega. clear Heqle_loop. subst.
+                sstep. rewrite Hloop in Hnow. inv Hnow.
+                split_and; first[reflexivity|solve_proof_low].
+              * intro CC. inversion CC. }
+        assert (Pre: P le_loop (m, d)) by (split; reflexivity).
+        pose proof (LoopProofSimpleWhile.termination _ _ _ _ _ _ T _ (m, d) Pre) as LoopProof.
+        destruct LoopProof as (le' & m' & (exec & Post)).
+        unfold exec_stmt in exec. rewrite Heqle_loop in exec.
+        unfold Q in Post. destruct Post as (Post & Hle'). rewrite Post in exec.
+
+        eexists. repeat big_vcgen.
+        solve_func64 z0. reflexivity.
+        symmetry. repeat sstep. assumption. somega. somega.
+        solve_func64 z2. reflexivity.
+        symmetry. repeat sstep.
+        solve_func z3. reflexivity.
+        symmetry. sstep. assumption. somega. somega. somega. somega.
+        solve_proof_low. simpl.
+        solve_proof_low.
+      Qed.
+
+
+
   End BodyProof.
 
 End CodeProof.
